tests/micro-benchmarks/Unit1.WPsAndTriples.fst
@@ -22,7 +22,9 @@ assume val as_Pure: #a:Type -> #b:(a -> Type)
           -> x:a -> Pure (b x) (as_requires (wp x))
                              (as_ensures (wp x))
 
-val f : x:int -> PURE int (fun 'p -> x > 0 /\ 'p (x + 1)) 
+open FStar.Monotonic.Pure
+
+val f : x:int -> PURE int (coerce_to_pure_wp (fun 'p -> x > 0 /\ 'p (x + 1)))
 let f x = assert (x > 0); x + 1
 
 val h : #req:(int -> Type) -> #ens:(int -> int -> Type) -> $f:(x:int -> Pure int (req x) (ens x)) -> y:int -> Pure int (req y) (ens y)
@@ -43,5 +45,5 @@ val bad_wp : unit -> PURE unit (fun p -> ~ (p ()))
 val bad_wp : unit -> PURE int (fun p -> ~ (p 3))
 
 
-val good_wp : unit -> PURE int (fun p -> p 3)
+val good_wp : unit -> PURE int (coerce_to_pure_wp (fun p -> p 3))
 val good_hoare : unit -> Pure int True (fun r -> r == 3)
